src/crypto/aes/ctr_clean.s.dfy
@@ -17,19 +17,18 @@ import opened dafny_wrappers_i
 import opened AESModule
 import opened AESHelpersModule
 
-datatype Pair<T,U> = Pair(0: T,1: U)
+// Use a ghost var of G, for ghosts, to cut the size of the code.
 datatype G = G(ghost key : seq<uint32>,
                ghost key_heap : heaplet_id,
-               ghost expanded_key : seq<uint32>,
-               ghost expanded_key_heap : heaplet_id,
+               ghost exp_key : seq<uint32>,
+               ghost exp_key_heap : heaplet_id,
                ghost iv       : uint64,
-               ghost input :seq<Quadword>,
-               ghost input_end  : uint64,
-               ghost input_heap : heaplet_id,
-               ghost output_heap : heaplet_id,
+               ghost inp :seq<Quadword>,
+               ghost inp_end  : uint64,
+               ghost inp_heap : heaplet_id,
+               ghost out_heap : heaplet_id,
                ghost alg: Algorithm,
-               ghost mem : Heaplets,
-               ghost old_mem : Heaplets)
+               ghost init_ctr : uint64)
 
 // We need to translate Quadwords to uint128 and versa vice.
 
@@ -67,10 +66,34 @@ function LowUint128(u : uint128) : uint64
  ((u % 0x1_00000000_00000000) as uint64)
 }
 
+predicate is_reg_edi(r : operand) {
+  r.OReg? && r == OReg(X86Edi)
+}
+
+// Bind the registers, passed as operators, to a physical register.
+predicate BindRegsPhy1(key_ptr : operand, exp_key_ptr : operand, iv_reg : operand, inp_ptr : operand, inp_end_ptr : operand,  out_ptr : operand, ctr_reg : operand, init_ctr : operand) {
+ key_ptr.OReg?      && key_ptr     == OReg(X86Edi) &&
+ exp_key_ptr.OReg?  && exp_key_ptr == OReg(X86Esi) && 
+ iv_reg.OReg?       && iv_reg      == OReg(X86Edx) && 
+ inp_ptr.OReg?      && inp_ptr     == OReg(X86Ecx) && 
+ inp_end_ptr.OReg?  && inp_end_ptr == OReg(X86R8) &&
+ out_ptr.OReg?      && out_ptr     == OReg(X86R9) &&
+ ctr_reg.OReg?      && ctr_reg     == OReg(X86Xmm(4)) &&
+ init_ctr.OReg?     && init_ctr    == OReg(X86R12) 
+}
+
+predicate BindRegsPhy1Curr(key_ptr : operand, exp_key_ptr : operand, iv_reg : operand, 
+                           inp_ptr : operand, inp_end_ptr : operand,  
+                           out_ptr : operand, ctr_reg : operand,
+                           init_ctr : operand,
+                           curr_inp_ptr : operand, curr_out_ptr : operand) {
+  BindRegsPhy1(key_ptr, exp_key_ptr, iv_reg, inp_ptr, inp_end_ptr, out_ptr, ctr_reg, init_ctr) && 
+  curr_inp_ptr.OReg? && curr_inp_ptr  == OReg(X86R10) &&   
+  curr_out_ptr.OReg? && curr_out_ptr == OReg(X86R11)
+}
+
 // Memory
-//  Only writing one heap and only from one pointer in a quadword heap
-//  and only count worth of N bytes.
-predicate Mem128ChangedOnlyIn(regptr : uint128, count : int, heap : heaplet_id, mem : Heaplets, oldmem: Heaplets)
+predicate Mem128ChangedOnlyIn(regptr : uint64, count : int, heap : heaplet_id, mem : Heaplets, oldmem: Heaplets)
 {
     heap in mem &&
     mem == oldmem[heap := mem[heap]] &&
@@ -100,36 +123,12 @@ predicate QuadwordSeqInMemory(qws : seq<Quadword>, mem: Heaplet, ptr : uint64)
     forall b:int :: 0 <= b < |qws| ==> ptr + b*16 in mem.quads && mem.quads[ptr + b*16].v == qws[b]  
 }
 
-// Memory
-
-
-// Ctr is in a register.
-predicate CtrInReg(ctr : Quadword, reg : Quadword) {
-  ctr == reg
-}
-
 predicate CtrInMem(ctr : Quadword, regptr : uint64, heap : heaplet_id, mem : Heaplets) { 
   // That register's value points to a readable source addresss in that heap with public taint.
   ValidSrcAddr(mem, heap, regptr, 128, Public) &&
   mem[heap].QuadwordHeaplet? &&
   ctr == mem[heap].quads[regptr].v
 }
-
-// An incremented counter has the high half undisturbed as it is the IV and
-// the low half + 1 with no overflow beyond 64 bits.
-predicate IncrCtr(counter : Quadword, incrcounter : Quadword)
-{
-  //counter.hi == incrcounter.hi &&
-  //counter.mid_hi == incrcounter.mid_hi
-  // No predicate provable.
-  true
-}
-  
-predicate IncrCtrInReg(ctr : Quadword, incctr : Quadword, reg : Quadword) {
-  IncrCtr(ctr, incctr) &&
-  CtrInReg(incctr, reg)
-}
-
 
 predicate AlgReq(alg : Algorithm, key : seq<uint32>, key_ptr : uint64) {
   alg == AES_128 &&
@@ -140,184 +139,126 @@ predicate AlgReq(alg : Algorithm, key : seq<uint32>, key_ptr : uint64) {
   key_ptr % 16 == 0
 }
 
-predicate HeapReq(key_heap : heaplet_id, expanded_key_heap : heaplet_id, input_heap : heaplet_id, output_heap : heaplet_id, mem : Heaplets) {
+predicate HeapReq(key_heap : heaplet_id, exp_key_heap : heaplet_id, inp_heap : heaplet_id, out_heap : heaplet_id, mem : Heaplets, old_mem : Heaplets) {
 // In the memory
-  key_heap in mem &&
-  expanded_key_heap in mem &&
-  input_heap in mem &&
-  output_heap in mem &&
+  key_heap in mem &&  exp_key_heap in mem &&  inp_heap in mem &&  out_heap in mem &&
+  key_heap in old_mem &&  exp_key_heap in old_mem &&  inp_heap in old_mem &&  out_heap in old_mem &&
 
 // Disjointness.
-  key_heap != expanded_key_heap &&
-  key_heap != input_heap &&
-  key_heap != output_heap &&
-  expanded_key_heap != input_heap &&
-  expanded_key_heap != output_heap &&
-  input_heap != output_heap
+  key_heap != exp_key_heap &&
+  key_heap != inp_heap &&
+  key_heap != out_heap &&
+  exp_key_heap != inp_heap &&
+  exp_key_heap != out_heap &&
+  inp_heap != out_heap &&
+
+// Types of heaplets in memory.
+  mem[inp_heap].QuadwordHeaplet? &&
+  mem[out_heap].QuadwordHeaplet? &&
+
+// Heaplets don't change.
+  mem[key_heap]    == old_mem[key_heap] &&
+  mem[exp_key_heap] == old_mem[exp_key_heap] &&
+  mem[inp_heap] == old_mem[inp_heap]
 }
+
 
 predicate KeyReq(key : seq<uint32>, key_heap : heaplet_id, key_ptr : uint64, mem : Heaplets) {
   ValidSrcAddrs(mem, key_heap, key_ptr, 128, Secret, 11*16) &&   // Key is readable
   key_ptr % 16 == 0
 }
 
-predicate ExpandedKeyInitReq(expanded_key : seq<uint32>, expanded_key_heap : heaplet_id,
-                             expanded_key_ptr : uint64, mem : Heaplets) {
-  SeqLength(expanded_key) == 44 &&
-  ValidSrcAddrs(mem, expanded_key_heap, expanded_key_ptr, 1, Secret, 176)
+predicate ExpKeyInitReq(exp_key : seq<uint32>, exp_key_heap : heaplet_id,
+                             exp_key_ptr : uint64, mem : Heaplets) {
+  SeqLength(exp_key) == 44 &&
+  ValidSrcAddrs(mem, exp_key_heap, exp_key_ptr, 1, Secret, 176)
 }
 
-predicate ExpandedKeyReq(key : seq<uint32>, key_heap : heaplet_id, key_ptr : uint64, expanded_key : seq<uint32>, expanded_key_heap : heaplet_id,
-                             expanded_key_ptr : uint64, mem : Heaplets, alg : Algorithm) {
+predicate ExpKeyReq(key : seq<uint32>, key_heap : heaplet_id, key_ptr : uint64, exp_key : seq<uint32>, exp_key_heap : heaplet_id,
+                             exp_key_ptr : uint64, mem : Heaplets, alg : Algorithm) {
   AlgReq(alg, key, key_ptr) &&
   KeyReq(key, key_heap, key_ptr, mem) && 
-  ExpandedKeyInitReq(expanded_key, expanded_key_heap, expanded_key_ptr, mem) && // Someday we may call this in assembly.
+  ExpKeyInitReq(exp_key, exp_key_heap, exp_key_ptr, mem) && // Someday we may call this in assembly.
    (forall j :: 0 <= j <= 10 ==> mem[key_heap].quads[key_ptr + 16*j].v == 
-         Quadword(expanded_key[4*j], expanded_key[4*j+1], expanded_key[4*j+2], expanded_key[4*j+3])) &&
-    KeyExpansionPredicate(key, alg, expanded_key)
+         Quadword(exp_key[4*j], exp_key[4*j+1], exp_key[4*j+2], exp_key[4*j+3])) &&
+    KeyExpansionPredicate(key, alg, exp_key)
 }
 
-predicate InputInMem(input : seq<Quadword>, input_heap : heaplet_id, input_ptr : uint64, 
-                    input_end : uint64, input_end_ptr : uint64, mem : Heaplets) {
-  SeqLength(input) > 0 &&
-  ValidSrcAddrs(mem, input_heap, input_ptr, 128, Secret, SeqLength(input)*16) &&
-  QuadwordSeqInMemory(input, mem[input_heap], input_ptr)
+predicate InpInMem(inp : seq<Quadword>, inp_heap : heaplet_id, inp_ptr : uint64, 
+                   inp_end : uint64, inp_end_ptr : uint64, mem : Heaplets) {
+  SeqLength(inp) > 0 &&
+  ValidSrcAddrs(mem, inp_heap, inp_ptr, 128, Secret, SeqLength(inp)*16) &&
+  QuadwordSeqInMemory(inp, mem[inp_heap], inp_ptr)
 }
 
-predicate OutputWriteable(output : seq<Quadword>, output_heap : heaplet_id, 
-                      output_ptr : uint64, mem : Heaplets) {
-  SeqLength(output) > 0 &&
-  ValidSrcAddrs(mem, output_heap, output_ptr, 128, Secret, SeqLength(output)*16)
+predicate OutWriteable(inp : seq<Quadword>, out_heap : heaplet_id, 
+                       out_ptr : uint64, mem : Heaplets) {
+  ValidSrcAddrs(mem, out_heap, out_ptr, 128, Secret, SeqLength(inp)*16)
 }
 
-// TODO
-// I abstractly know what my starting counter is. 
-predicate StartCtrReq(iv : uint64, ctr : Quadword) {
-  //ctr == Quadword(0,0,lower64(iv), upper64(iv))
-  true
+predicate InpOutInvariants(inp : seq<Quadword>, inp_ptr : uint64, inp_end_ptr : uint64, 
+                               out_ptr : uint64) {
+   inp_ptr + SeqLength(inp)*16 < 0x1_0000_0000_0000_0000 &&
+   out_ptr + SeqLength(inp)*16 < 0x1_0000_0000_0000_0000 &&
+   inp_end_ptr >= inp_ptr && 
+   inp_end_ptr == inp_ptr + SeqLength(inp)*16 &&
+   inp_end_ptr < 0x1_0000_0000_0000_0000 
 }
 
-// I concretely know.
-predicate StartCtrInReg(iv : uint64, ctr : Quadword, ctr_reg : Quadword) {
- //StartCtrReq(iv, ctr) // &&
-  //ctr == ctr_reg
-// TODO
-  // Error: cannot establish the existence of LHS values that satisfy the such-that predicate
- true
-}
-
-predicate InputOutputInvariants(input : seq<Quadword>, input_ptr : uint64, input_end_ptr : uint64, 
-                               output_ptr : uint64) {
-   input_ptr + SeqLength(input)*16 < 0x1_0000_0000_0000_0000 &&
-   output_ptr + SeqLength(input)*16 < 0x1_0000_0000_0000_0000 &&
-   input_end_ptr >= input_ptr && 
-   input_end_ptr == input_ptr + SeqLength(input)*16 &&
-   input_end_ptr < 0x1_0000_0000_0000_0000 
-}
-
-predicate CTRInvariants(
-    key     : seq<uint32>,
-    key_ptr : uint64,
-    key_heap : heaplet_id,
-    expanded_key : seq<uint32>,
-    expanded_key_ptr : uint64,
-    expanded_key_heap : heaplet_id,
-    iv       : uint64,
-    input :seq<Quadword>,
-    input_ptr : uint64,
-    input_end  : uint64,
-    input_end_ptr : uint64,
-    input_heap : heaplet_id,
-    output_heap : heaplet_id,
-    output_ptr : uint64,
-    alg: Algorithm,
-    mem : Heaplets,
+predicate CTRInv(g : G,
+    key_ptr : uint64, exp_key_ptr : uint64,
+    inp_ptr : uint64, inp_end_ptr : uint64,
+    out_ptr : uint64,
+    mem : Heaplets, 
     old_mem : Heaplets)
 {
-        HeapReq(key_heap, expanded_key_heap, input_heap, output_heap, mem) &&
-        KeyReq(key, key_heap, key_ptr, mem) &&
-        ExpandedKeyReq(key, key_heap, key_ptr, expanded_key, expanded_key_heap,
-                            expanded_key_ptr, mem, alg) &&
-        InputInMem(input, input_heap, input_ptr, input_end, input_end_ptr, mem) &&
-        OutputWriteable(input, output_heap, output_ptr, mem) &&
-        InputOutputInvariants(input, input_ptr, input_end_ptr, output_ptr) &&
-        mem == old_mem[output_heap := mem[output_heap]]
+        HeapReq(g.key_heap, g.exp_key_heap, g.inp_heap, g.out_heap, mem, old_mem) &&
+        KeyReq(g.key, g.key_heap, key_ptr, mem) &&
+        ExpKeyReq(g.key, g.key_heap, key_ptr, g.exp_key, g.exp_key_heap,
+                            exp_key_ptr, mem, g.alg) &&
+        InpInMem(g.inp, g.inp_heap, inp_ptr, g.inp_end, inp_end_ptr, mem) &&
+        OutWriteable(g.inp, g.out_heap, out_ptr, mem) &&
+        InpOutInvariants(g.inp, inp_ptr, inp_end_ptr, out_ptr) &&
+        mem == old_mem[g.out_heap := mem[g.out_heap]]
 }
 
 
-predicate CTROutputFinal2(key : seq<uint32>, input :seq<Quadword>, iv : uint64, alg : Algorithm, 
-                         mem : Heaplets,  output_heap : heaplet_id, output_ptr :uint64, output : seq<Quadword>, ctr : Quadword) {
-  true
-}
-
-predicate CTREncryptLoopInvariant(
-    key     : seq<uint32>,
-    key_ptr : uint64,
-    key_heap : heaplet_id,
-    expanded_key : seq<uint32>,
-    expanded_key_ptr : uint64,
-    expanded_key_heap : heaplet_id,
-    iv       : uint64,
-    input :seq<Quadword>,
-    input_ptr : uint64,
-    input_end  : uint64,
-    input_end_ptr : uint64,
-    input_heap : heaplet_id,
-    output_heap : heaplet_id,
-    output_ptr : uint64,
-    alg: Algorithm,
-    mem : Heaplets,
-    old_mem : Heaplets,
-    iteration : nat) {
-  CTRInvariants(key, key_ptr, key_heap, expanded_key, expanded_key_ptr, expanded_key_heap, iv,
-          input, input_ptr, input_end, input_end_ptr, input_heap, output_heap, output_ptr, alg, 
-          mem, old_mem)
-}
-
-lemma lemma_CTREncryptInvarientImplications(input : seq<Quadword>)
-  returns (output : seq<Quadword>) {
-    output := input;
-}
-
-predicate CTREncryptBodyPreconditions() {
-  true
-}
-
-predicate CTREncryptBodyPostconditions() {
-  true
-}
-
+// Can't make the last requirement work due to a bug in Vale or Dafney.
+//predicate ChangeOnly1Block(inp_ptr : uint64,   inp_heap : heaplet_id, 
+//                           out_ptr : uint64,   out_heap : heaplet_id,
+//                           mem     : Heaplets, old_mem  : Heaplets, iteration : nat) 
+//// An awful lot of requirements to move a simple thing into dafny.
+//   requires out_heap in mem;                           
+//   requires mem[out_heap].QuadwordHeaplet?;
+//   requires out_heap in old_mem;
+//   requires old_mem[out_heap].QuadwordHeaplet?;
+//   requires inp_heap in mem;
+//   requires mem[inp_heap].QuadwordHeaplet?;
+////   requires (inp_ptr+(iteration*16)) in mem[inp_heap];
+//{
+//     mem == old_mem[out_heap := mem[out_heap]] &&
+//     mem[out_heap].quads == 
+//     (old_mem[out_heap].quads)
+//     [out_ptr+(iteration*16) := mem[inp_heap].quads[inp_ptr+(iteration*16)]]
+//}                            
 
 // Just for learning how to write the code/proofs.
 
 predicate QuadwordSeqsInMemMatch
-  (input  : seq<Quadword>, in_mem  : Heaplet, input_ptr : uint64,
-   output : seq<Quadword>, out_mem : Heaplet, output_ptr : uint64,
+  (inp  : seq<Quadword>, in_mem  : Heaplet, inp_ptr : uint64,
+   out : seq<Quadword>, out_mem : Heaplet, out_ptr : uint64,
    length : int)
   requires in_mem.QuadwordHeaplet?
   requires out_mem.QuadwordHeaplet?
 {
-  |input| == |output| &&
-  |input| >= length &&
+  |inp| == |out| &&
+  |inp| >= length &&
    forall b:int :: 0 <= b < length ==> 
-     input_ptr  + b*16 in in_mem.quads && 
-     output_ptr + b*16 in out_mem.quads && 
-     in_mem.quads[input_ptr + b*16].v == out_mem.quads[output_ptr + b*16].v
+     inp_ptr  + b*16 in in_mem.quads && 
+     out_ptr + b*16 in out_mem.quads && 
+     in_mem.quads[inp_ptr + b*16].v == out_mem.quads[out_ptr + b*16].v
 }
 
-
-predicate InputCopied
-  (in_mem  : Heaplet, input_ptr : uint64,
-   out_mem : Heaplet, output_ptr : uint64,
-   position : int)
-  requires in_mem.QuadwordHeaplet?
-  requires out_mem.QuadwordHeaplet?
-{
-  input_ptr  + position*16 in in_mem.quads && 
-  output_ptr + position*16 in out_mem.quads && 
-  in_mem.quads[input_ptr + position*16].v == out_mem.quads[output_ptr + position*16].v
-}
 
 // End of Module
-
 }
